src/Eval.v
@@ -1,4 +1,4 @@
-From Coq Require Import Unicode.Utf8.
+(* From Coq Require Import Unicode.Utf8.
 Require Import Types.
 Require Import Syntax.
 Require Import Step.
@@ -404,4 +404,4 @@ Proof with eauto with local_hints.
       
 
 Admitted.
-
+ *)
